theories/Dot/syn/pathrepl.v
@@ -5,108 +5,56 @@ From D.Dot.lr Require Import unary_lr.
 
 Implicit Types
          (T : ty) (v w : vl) (t : tm) (d : dm) (ds : dms) (p q : path)
-         (Γ : ctx) (vs : vls) (l : label).
-
-Implicit Types (Pv : vl → Prop).
+         (Γ : ctx) (vs : vls) (l : label) (Pv : vl → Prop).
 Set Nested Proofs Allowed.
-
-(* XXX For Iris *)
-Hint Extern 1 (environments.envs_entails _ (_ ∗-∗ _)) => iSplit : core.
 
 Lemma ren_scons v ρ : ren (+1) >> v .: ρ = ρ.
 Proof. done. Qed.
 
-Fixpoint path_wp_pure p Pv : Prop :=
-  match p with
-  | pself p l => path_wp_pure p (λ v, ∃ w, v @ l ↘ dvl w ∧ Pv w)
-  | pv vp => Pv vp
-  end.
-
-Global Instance Proper_pwp: Proper ((=) ==> pointwise_relation _ iff ==> iff) path_wp_pure.
-Proof.
-  (* The induction works best in this shape, but this instance is best kept local. *)
-  have Proper_pwp_2: ∀ p, Proper (pointwise_relation _ iff ==> iff) (path_wp_pure p).
-  elim; solve_proper.
-  solve_proper.
-Qed.
-
-Lemma path_wp_pure_wand {Pv1 Pv2 p}:
-  path_wp_pure p Pv1 →
-  (∀ v, Pv1 v → Pv2 v) →
-  path_wp_pure p Pv2.
-Proof.
-  elim: p Pv1 Pv2 => /= [v|p IHp l] Pv1 Pv2 Hp Hwand;
-    first by apply Hwand.
-  apply: (IHp _ _ Hp) => {IHp Hp} v [vq [??]].
-  eauto.
-Qed.
-
-Lemma path_wp_pure_eq p Pv :
-  path_wp_pure p Pv ↔ ∃ v, path_wp_pure p (λ w, w = v) ∧ Pv v.
-Proof.
-  elim: p Pv => [ v | p IHp l ] Pv /=; split.
-  - eauto.
-  - by destruct 1 as (w & <- & ?).
-  - rewrite IHp.
-    destruct 1 as (v & Hp & w & ?&?).
-    eexists w; split; last by [].
-    apply (path_wp_pure_wand Hp).
-    intros; subst; exists w; eauto.
-  - setoid_rewrite IHp; intros; ev; subst; eauto.
-Qed.
-
-Lemma path_wp_pure_det {p v1 v2}:
-  path_wp_pure p (λ w, w = v1) →
-  path_wp_pure p (λ w, w = v2) →
-  v1 = v2.
-Proof.
-  elim: p v1 v2 => [v /=| p /= IHp l //] v1 v2; first by intros <- <-.
-  rewrite !path_wp_pure_eq; intros (w1 & Hp1 & ?) (w2 & Hp2 & ?);
-    move: (IHp _ _ Hp1 Hp2) => ?; ev; simplify_eq.
-  by objLookupDet.
-Qed.
-
-Lemma path_wp_pure_swap p u :
-  path_wp_pure p (λ w, u = w) ↔
-  path_wp_pure p (λ w, w = u).
-Proof. split => Hp; exact: path_wp_pure_wand. Qed.
-
 (* XXX Unclear why is the substitution built-in. But beware of dropping that, as substitution and path replacement don't swap. *)
-Definition alias_paths_pure p q ρ :=
+Definition alias_paths p q ρ :=
   path_wp_pure p.|[ρ] (λ vp, path_wp_pure q.|[ρ] (λ vq, vp = vq)).
 
-Lemma alias_path_pure_weaken p q ρ v:
-  alias_paths_pure p.|[ren (+1)] q.|[ren (+1)] (v .: ρ) ↔
-  alias_paths_pure p q ρ.
-Proof.
-  by rewrite /alias_paths_pure; f_equiv; rewrite hsubst_comp ren_scons.
-Qed.
-
-Lemma alias_paths_pure_refl_vl v ρ :
-  alias_paths_pure (pv v) (pv v) ρ.
+Lemma alias_paths_pv_eq_1 p vr ρ :
+  alias_paths p (pv vr) ρ ↔ path_wp_pure p.|[ρ] (λ w, w = vr.[ρ]).
 Proof. done. Qed.
 
-Lemma alias_paths_pure_eq p q ρ:
-  alias_paths_pure p q ρ ↔
+Lemma alias_paths_pv_eq_2 p vr ρ :
+  alias_paths (pv vr) p ρ ↔ path_wp_pure p.|[ρ] (λ w, w = vr.[ρ]).
+Proof. by rewrite -path_wp_pure_swap. Qed.
+
+Lemma alias_paths_weaken p q ρ v:
+  alias_paths p.|[ren (+1)] q.|[ren (+1)] (v .: ρ) =
+  alias_paths p q ρ.
+Proof.
+  by rewrite /alias_paths; f_equiv; rewrite hsubst_comp ren_scons.
+Qed.
+
+Lemma alias_paths_refl_vl v ρ :
+  alias_paths (pv v) (pv v) ρ.
+Proof. done. Qed.
+
+Lemma alias_paths_sameres p q ρ:
+  alias_paths p q ρ ↔
   ∃ v,
     path_wp_pure p.|[ρ] (λ vp, vp = v) ∧
     path_wp_pure q.|[ρ] (λ vq, vq = v).
 Proof.
-  rewrite /= /alias_paths_pure !path_wp_pure_eq. split => -[vp];
+  rewrite /= /alias_paths !path_wp_pure_eq. split => -[vp];
     [ rewrite (path_wp_pure_swap q.|[_]) |
       rewrite -(path_wp_pure_swap q.|[_]) ]; eauto.
 Qed.
 
-Lemma alias_paths_pure_symm p q ρ :
-  alias_paths_pure p q ρ → alias_paths_pure q p ρ.
-Proof. rewrite !alias_paths_pure_eq. intros; ev; eauto. Qed.
+Lemma alias_paths_symm p q ρ :
+  alias_paths p q ρ → alias_paths q p ρ.
+Proof. rewrite !alias_paths_sameres. intros; ev; eauto. Qed.
 
 Lemma alias_paths_equiv_pure p q ρ:
-  alias_paths_pure p q ρ ↔
+  alias_paths p q ρ ↔
     (∃ u, path_wp_pure p.|[ρ] (λ vp, vp = u)) ∧
     ∀ Pv, path_wp_pure p.|[ρ] Pv ↔ path_wp_pure q.|[ρ] Pv.
 Proof.
-  rewrite alias_paths_pure_eq; split.
+  rewrite alias_paths_sameres; split.
   - destruct 1 as (v & Hp & Hq).
     split. by eauto. intros Pv.
     rewrite !path_wp_pure_eq.
@@ -116,131 +64,6 @@ Proof.
   - intros [[u Hp] Heq]. exists u.
     split; by [|rewrite -Heq].
 Qed.
-
-Section equivI_utils.
-  Context `{dlangG Σ}.
-
-  Lemma exists_equivI {A} {PROP: sbi} (φ1 φ2 : A -d> PROP) :
-    (∀ x, φ1 x ≡ φ2 x) ⊢@{PROP}
-    (∃ x, φ1 x) ≡ ∃ x, φ2 x.
-  Proof.
-    rewrite -discrete_fun_equivI.
-    apply (@f_equiv _ _ _ (λ φ : _ -d> _, ∃ x, φ x)%I). solve_proper.
-  Qed.
-
-  Lemma forall_equivI {A} {PROP: sbi} (φ1 φ2 : A -d> PROP) :
-    (∀ x, φ1 x ≡ φ2 x) ⊢@{PROP}
-    (∀ x, φ1 x) ≡ ∀ x, φ2 x.
-  Proof.
-    rewrite -discrete_fun_equivI.
-    apply (@f_equiv _ _ _ (λ φ : _ -d> _, ∀ x, φ x)%I). solve_proper.
-  Qed.
-
-  Lemma wp_equivI (φ1 φ2 : vl -d> iPropO Σ) t :
-    (∀ x, φ1 x ≡ φ2 x) ⊢@{iPropI Σ}
-    WP t {{ φ1 }} ≡ WP t {{ φ2 }}.
-  Proof.
-    rewrite -discrete_fun_equivI.
-    apply (@f_equiv _ _ _ (λ φ : _ -d> _, WP t {{ φ }})%I). solve_proper.
-  Qed.
-
-  Lemma or2_equivI {PROP : sbi} (P1 P2 Q : PROP) :
-    P1 ≡ P2 ⊢@{PROP} (P1 ∨ Q) ≡ (P2 ∨ Q).
-  Proof. apply (@f_equiv _ _ _ (λ P, P ∨ Q)%I). solve_proper. Qed.
-
-  Lemma and2_equivI {PROP : sbi} (P1 P2 Q : PROP) :
-    P1 ≡ P2 ⊢@{PROP} (P1 ∧ Q) ≡ (P2 ∧ Q).
-  Proof. apply (@f_equiv _ _ _ (λ P, P ∧ Q)%I). solve_proper. Qed.
-
-  Lemma wand2_equivI {PROP : sbi} (P1 P2 Q : PROP) :
-    P1 ≡ P2 ⊢@{PROP} (P1 -∗ Q) ≡ (P2 -∗ Q).
-  Proof. apply (@f_equiv _ _ _ (λ P, P -∗ Q)%I). solve_proper. Qed.
-
-End equivI_utils.
-
-Ltac iProperness :=
-  repeat first
-  [ iEval (progress rewrite -(wp_equivI, exists_equivI, forall_equivI)); iIntros
-  (* f_equiv must come before those others for performance. *)
-  | iEval (progress rewrite -(f_equiv, and2_equivI, wand2_equivI, or2_equivI))
-  ].
-
-Section path_repl.
-  Context `{dlangG Σ}.
-  Implicit Types (φ: vl → iProp Σ).
-
-  Notation path_wp p φ := (@path_wp Σ p φ).
-  Notation path_wp_purel p Pv := (⌜path_wp_pure p Pv⌝%I : iProp Σ).
-
-  Lemma path_wp_pureable p Pv:
-    path_wp p (λ v, ⌜Pv v⌝) ⊣⊢ path_wp_purel p Pv.
-  Proof.
-    elim: p Pv => /= [//|p IHp l] Pv.
-    by rewrite -{}IHp; f_equiv => v; iIntros "!% /=".
-  Qed.
-
-  Global Instance path_wp_pureableI p Pv :
-    IntoPure (path_wp p (λ v, ⌜Pv v⌝))%I (path_wp_pure p Pv).
-  Proof. by rewrite /IntoPure path_wp_pureable. Qed.
-  Global Instance path_wp_pureableF p Pv :
-    FromPure false (path_wp p (λ v, ⌜Pv v⌝))%I (path_wp_pure p Pv).
-  Proof. by rewrite /FromPure/= path_wp_pureable. Qed.
-
-  Lemma path_wp_swap p u :
-    path_wp p (λ w, ⌜u = w⌝) ⊣⊢ path_wp p (λ w, ⌜w = u⌝).
-  Proof. iIntros "!%". by rewrite /= path_wp_pure_swap. Qed.
-
-  Definition alias_paths p q ρ : iProp Σ := ⌜alias_paths_pure p q ρ⌝.
-
-  Lemma alias_paths_refl_vl v ρ :
-    alias_paths (pv v) (pv v) ρ.
-  Proof. by iIntros "!%". Qed.
-
-  Lemma alias_paths_eq p q ρ:
-    alias_paths p q ρ ⊣⊢
-    ∃ v,
-      path_wp p.|[ρ] (λ vp : vl, ⌜vp = v⌝) ∧
-      path_wp q.|[ρ] (λ vq : vl, ⌜vq = v⌝).
-  Proof. iIntros "!%"; rewrite /= alias_paths_pure_eq. intuition. Qed.
-
-  Lemma simpl_alias_1 p vr ρ :
-    alias_paths p (pv vr) ρ ⊣⊢ path_wp_purel p.|[ρ] (λ w, w = vr.[ρ]).
-  Proof. done. Qed.
-
-  Lemma simpl_alias_2 p vr ρ :
-    alias_paths (pv vr) p ρ ⊣⊢ path_wp_purel p.|[ρ] (λ w, w = vr.[ρ]) .
-  Proof. by rewrite -path_wp_pure_swap. Qed.
-
-  (* Not provable through pure props for impure [φ]. *)
-  Lemma alias_paths_equiv p q ρ:
-    alias_paths_pure p q ρ ↔
-      (∃ u, path_wp_pure p.|[ρ] (λ vp, vp = u)) ∧
-      ∀ φ, path_wp p.|[ρ] φ ≡ path_wp q.|[ρ] φ.
-  Proof.
-    rewrite alias_paths_pure_eq; split.
-    - destruct 1 as (v & Hp & Hq).
-      split; first by [eauto]; intros φ.
-      rewrite !path_wp_eq. f_equiv => w.
-      rewrite !path_wp_pureable; do 2 f_equiv.
-      split => Hr; [ rewrite -(path_wp_pure_det Hp Hr)
-        | rewrite -(path_wp_pure_det Hq Hr)]; auto.
-    - destruct 1 as ((u & Hp) & Heq). exists u; split; first done.
-      (* Yes, completely insane. *)
-      apply (pure_soundness (M := iResUR Σ)).
-      iRevert (Hp). by rewrite -!path_wp_pureable Heq.
-  Qed.
-
-  Lemma alias_paths_equiv' p q ρ:
-    alias_paths p q ρ ⊣⊢
-      (∃ u, path_wp p.|[ρ] (λ vp, ⌜vp = u⌝)) ∧
-      ∀ φ, ⌜path_wp p.|[ρ] φ ≡ path_wp q.|[ρ] φ⌝.
-  Proof. iIntros "!%". apply alias_paths_equiv. Qed.
-
-  Lemma alias_paths_elim_eq φ p q ρ:
-    alias_paths_pure p q ρ →
-    path_wp p.|[ρ] φ ≡ path_wp q.|[ρ] φ.
-  Proof. intros ?%alias_paths_equiv. intuition. Qed.
-End path_repl.
 
 Reserved Notation "p1 ~pp[ p := q  ] p2" (at level 70).
 Inductive path_path_repl (p q : path) : path → path → Prop :=
@@ -252,7 +75,6 @@ where "p1 ~pp[ p := q  ] p2" := (path_path_repl p q p1 p2) .
 
 Lemma psubst_path_id p1 p2 p : p1 ~pp[ p := p ] p2 → p1 = p2.
 Proof. by elim; intros; simplify_eq/=. Qed.
-
 
 Reserved Notation "T1 ~p[ p := q  ] T2" (at level 70).
 
@@ -301,24 +123,52 @@ Proof.
   f_equiv; exact: psubst_path_id.
 Qed.
 
-Section path_repl_2.
+(* XXX For Iris *)
+Hint Extern 1 (environments.envs_entails _ (_ ∗-∗ _)) => iSplit : core.
+
+Definition alias_pathsI {Σ} p q ρ : iProp Σ := ⌜alias_paths p q ρ⌝.
+
+Section path_repl.
   Context `{dlangG Σ}.
   Implicit Types (φ: vl → iProp Σ).
 
   Notation path_wp p φ := (@path_wp Σ p φ).
-  Notation path_wp_purel p Pv := (⌜path_wp_pure p Pv⌝%I : iProp Σ).
-  Notation alias_paths p q ρ := (@alias_paths Σ p q ρ).
+  Notation alias_pathsI p q ρ := (@alias_pathsI Σ p q ρ).
+
+  (* Not provable through pure props for impure [φ]. *)
+  Lemma alias_paths_samepwp p q ρ:
+    alias_paths p q ρ ↔
+      (∃ u, path_wp_pure p.|[ρ] (λ vp, vp = u)) ∧
+      ∀ φ, path_wp p.|[ρ] φ ≡ path_wp q.|[ρ] φ.
+  Proof.
+    rewrite alias_paths_sameres; split.
+    - destruct 1 as (v & Hp & Hq).
+      split; first by [eauto]; intros φ.
+      rewrite !path_wp_eq. f_equiv => w.
+      rewrite !path_wp_pureable; do 2 f_equiv.
+      split => Hr; [ rewrite -(path_wp_pure_det Hp Hr)
+        | rewrite -(path_wp_pure_det Hq Hr)]; auto.
+    - destruct 1 as ((u & Hp) & Heq). exists u; split; first done.
+      (* Yes, completely insane. *)
+      apply (pure_soundness (M := iResUR Σ)).
+      iRevert (Hp). by rewrite -!path_wp_pureable Heq.
+  Qed.
+
+  Lemma alias_paths_elim_eq φ p q ρ:
+    alias_paths p q ρ →
+    path_wp p.|[ρ] φ ≡ path_wp q.|[ρ] φ.
+  Proof. intros ?%alias_paths_samepwp. intuition. Qed.
 
   (** Beware: we can do path replacement *before* substitution,
       even tho substitution and path replacement don't commute nicely.
 
       As a special case, we get the less surprising:
-      [alias_paths_pure p r ids → path_wp q φ ≡ path_wp (q .p[p := r]) φ].
+      [alias_paths p r ids → path_wp q φ ≡ path_wp (q .p[p := r]) φ].
 
       But we do need the general form. *)
   Lemma path_replacement_equiv {p r ρ} q q' (φ : vl → iProp Σ):
     q ~pp[ p := r ] q' →
-    alias_paths_pure p r ρ →
+    alias_paths p r ρ →
     path_wp q.|[ρ] φ ≡ path_wp q'.|[ρ] φ.
   Proof.
     move => Hrepl.
@@ -329,19 +179,13 @@ Section path_repl_2.
 
   Lemma rewrite_ty_path_repl p q T1 T2 ρ v:
     T1 ~p[ p := q ] T2 →
-    alias_paths_pure p q ρ → (* p : q.type *)
+    alias_paths p q ρ → (* p : q.type *)
     ⟦ T1 ⟧ ρ v ≡ ⟦ T2 ⟧ ρ v.
   Proof.
     move => Hrew; move: v ρ.
     induction Hrew => v ρ He /=; properness;
-      by [|exact: path_replacement_equiv|iApply IHHrew; rewrite ?alias_path_pure_weaken].
+      by [|exact: path_replacement_equiv|iApply IHHrew; rewrite ?alias_paths_weaken].
   Qed.
-
-  Lemma rewrite_ty_path_repl' p q T1 T2 ρ v:
-    T1 ~p[ p := q ] T2 →
-    alias_paths p q ρ ⊢
-    ⟦ T1 ⟧ ρ v ≡ ⟦ T2 ⟧ ρ v.
-  Proof. iIntros "!%". exact: rewrite_ty_path_repl. Qed.
 
   (* Lemma TMu_E Γ T v: Γ ⊨ tv v : TMu T -∗ Γ ⊨ tv v : T.|[ids 0/] .p [.
   Proof. by rewrite TMu_equiv. Qed.
@@ -349,4 +193,4 @@ Section path_repl_2.
   Lemma TMu_I Γ T v: Γ ⊨ tv v : T.|[v/] -∗ Γ ⊨ tv v : TMu T.
   Proof. by rewrite TMu_equiv. Qed. *)
 
-End path_repl_2.
+End path_repl.
